repr/Test.v
@@ -9,8 +9,8 @@ Unset MetaCoq Strict Unquote Universe Mode.
 Instance repr_bytestring : Repr bytestring.string := 
 { repr_prec _ s := group $ bracket """" (str $ pstring_of_bytestring s) """" }.
 
-Instance repr_sort : Repr sort :=
-{ repr_prec _ _ := str "#sort" }.
+(*Instance repr_sort : Repr sort :=
+{ repr_prec _ _ := str "#sort" }.*)
 
 Instance repr_int63 : Repr int :=
 { repr_prec _ x := str $ pstring_of_nat $ to_nat x }.
@@ -18,19 +18,28 @@ Instance repr_int63 : Repr int :=
 Instance repr_float : Repr float :=
 { repr_prec _ _ := str "#float" }.
 
-MetaCoq Run (derive_global cast_kind).
-MetaCoq Run (derive_global name).
-MetaCoq Run (derive_global relevance).
-MetaCoq Run (derive_global binder_annot).
-MetaCoq Run (derive_global modpath).
-MetaCoq Run (derive_global Level.t_).
-MetaCoq Run (derive_global inductive).
-MetaCoq Run (derive_global case_info).
-MetaCoq Run (derive_global predicate).
-MetaCoq Run (derive_global branch).
-MetaCoq Run (derive_global def).
-MetaCoq Run (derive_global projection).
-MetaCoq Run (derive_global term).
+MetaCoq Run (derive_export cast_kind).
+MetaCoq Run (derive_export name).
+MetaCoq Run (derive_export relevance).
+MetaCoq Run (derive_export binder_annot).
+MetaCoq Run (derive_export modpath).
+MetaCoq Run (derive_export Level.t_).
+Instance repr_LevelExprSet_Raw_Ok {set} : Repr (LevelExprSet.Raw.Ok set) :=
+{ repr_prec _ _ := str "_" }.
+
+Instance repr_sort : Repr sort :=
+{ repr_prec _ _ := str "#sort" }.
+
+(*MetaCoq Run (derive_export LevelExprSet.t_).*)
+
+MetaCoq Run (derive_export inductive).
+MetaCoq Run (derive_export case_info).
+MetaCoq Run (derive_export predicate).
+MetaCoq Run (derive_export branch).
+MetaCoq Run (derive_export def).
+MetaCoq Run (derive_export projection).
+MetaCoq Run (derive_export term).
+
 
 
 (*MetaCoq Quote Definition big_def := 
